src/Std/Data/Iterators/Lemmas/Combinators/Monadic/StepSize.lean
@@ -1,0 +1,31 @@
+/-
+Copyright (c) 2026 Lean FRO, LLC. All rights reserved.
+Released under Apache 2.0 license as described in the file LICENSE.
+Authors: Paul Reichert
+-/
+module
+
+prelude
+public import Std.Data.Iterators.Combinators.Monadic.StepSize
+
+public section
+open Std Std.Iterators Std.Iterators.Types
+
+namespace Std.IterM
+
+-- example [Iterator α Id β] [IteratorAccess α Id] [LawfulDeterministicIterator α Id] :
+--     Productive α Id where
+--   wf := by
+--     constructor
+--     intro it
+--     have :=
+
+-- instance [Iterator α m β] [LawfulDeterministicIterator α m] [IteratorAccess α m] [Monad m] :
+--     LawfulDeterministicIterator (StepSizeIterator α m β) m where
+--   isPlausibleStep_eq_eq it := by
+--     simp only [IterM.IsPlausibleStep, Iterator.IsPlausibleStep, funext_iff]
+--     obtain ⟨⟨
+
+-- theorem step_stepSize
+
+end Std.IterM
