src/Std/Data/Iterators/Lemmas/Combinators/StepSize.lean
@@ -1,0 +1,175 @@
+/-
+Copyright (c) 2026 Lean FRO, LLC. All rights reserved.
+Released under Apache 2.0 license as described in the file LICENSE.
+Authors: Paul Reichert
+-/
+module
+
+prelude
+public import Init.Data.Iterators.Consumers.Access
+public import Init.Data.Iterators.Consumers.Collect
+public import Init.Data.Iterators.Combinators.Take
+public import Std.Data.Iterators.Combinators.StepSize
+import Init.Data.Iterators.Lemmas.Consumers.Access
+
+public section
+open Std Std.Iterators Std.Iterators.Types
+
+namespace Std.Iter
+
+-- example [Iterator α Id β] [IteratorAccess α Id] [LawfulDeterministicIterator α Id] :
+--     Productive α Id where
+--   wf := by
+--     constructor
+--     intro it
+--     have :=
+
+-- instance [Iterator α m β] [LawfulDeterministicIterator α m] [IteratorAccess α m] [Monad m] :
+--     LawfulDeterministicIterator (StepSizeIterator α m β) m where
+--   isPlausibleStep_eq_eq it := by
+--     simp only [IterM.IsPlausibleStep, Iterator.IsPlausibleStep, funext_iff]
+--     obtain ⟨⟨
+
+-- theorem step_stepSize
+
+instance [Iterator α Id β] [LawfulDeterministicIterator α Id] {it : IterM (α := α) Id β} :
+    Subsingleton it.Step where
+  allEq s s' := by
+    obtain ⟨s'', hs''⟩ := LawfulDeterministicIterator.isPlausibleStep_eq_eq it
+    obtain ⟨s, hs⟩ := s
+    obtain ⟨s', hs'⟩ := s'
+    simp only [hs''] at hs hs'
+    have := hs.trans hs'.symm
+    rwa [Subtype.mk.injEq]
+
+instance [Iterator α Id β] [LawfulDeterministicIterator α Id] {it : Iter (α := α) β} :
+    Subsingleton it.Step where
+  allEq s s' := by
+    obtain ⟨s'', hs''⟩ := LawfulDeterministicIterator.isPlausibleStep_eq_eq it.toIterM
+    obtain ⟨s, hs⟩ := s
+    obtain ⟨s', hs'⟩ := s'
+    simp only [Iter.IsPlausibleStep, hs''] at hs hs'
+    have := hs.trans hs'.symm
+    rw [IterStep.mapIterator_inj (fun _ _ => toIterM_inj.mp) ] at this
+    rwa [Subtype.mk.injEq]
+
+theorem eq_step_of_isPlausibleStep [Iterator α Id β] [LawfulDeterministicIterator α Id]
+    {it : Iter (α := α) β} {step} (h : it.IsPlausibleStep step) :
+    step = it.step.val := by
+  have : ⟨step, h⟩ = it.step := Subsingleton.allEq _ _
+  simp [← this]
+
+theorem _root_.Std.IterM.eq_step_of_isPlausibleStep [Iterator α Id β] [LawfulDeterministicIterator α Id]
+    {it : IterM (α := α) Id β} {step} (h : it.IsPlausibleStep step) :
+    step = it.step.run.inflate.val := by
+  have : ⟨step, h⟩ = it.step.run.inflate := Subsingleton.allEq _ _
+  simp [← this]
+
+theorem _root_.Std.IterM.eq_of_isPlausibleNthOutputStep_of_isPlausibleNthOutputStep [Iterator α Id β]
+    [LawfulDeterministicIterator α Id]
+    {it : IterM (α := α) Id β} {s s'}
+    (hs : it.IsPlausibleNthOutputStep n s)
+    (hs' : it.IsPlausibleNthOutputStep n s') :
+    s = s' := by
+  induction hs
+  case zero_yield h =>
+    match hs' with
+    | .zero_yield h' ..
+    | .skip h' ..
+    | .done h' =>
+      replace h := IterM.eq_step_of_isPlausibleStep h
+      replace h' := IterM.eq_step_of_isPlausibleStep h'
+      rw [← h] at h'
+      cases h'
+      all_goals rfl
+  case done h =>
+    match hs' with
+    | .zero_yield h' ..
+    | .yield h' ..
+    | .skip h' ..
+    | .done h' =>
+      replace h := IterM.eq_step_of_isPlausibleStep h
+      replace h' := IterM.eq_step_of_isPlausibleStep h'
+      rw [← h] at h'
+      all_goals cases h'
+      all_goals rfl
+  case yield h _ ih =>
+    match hs' with
+    | .yield h' ..
+    | .skip h' ..
+    | .done h' =>
+      replace h := IterM.eq_step_of_isPlausibleStep h
+      replace h' := IterM.eq_step_of_isPlausibleStep h'
+      rw [← h] at h'
+      cases h'
+      all_goals
+        apply ih ‹_›
+  case skip h _ ih =>
+    match hs' with
+    | .zero_yield h' ..
+    | .yield h' ..
+    | .skip h' ..
+    | .done h' =>
+      replace h := IterM.eq_step_of_isPlausibleStep h
+      replace h' := IterM.eq_step_of_isPlausibleStep h'
+      rw [← h] at h'
+      cases h'
+      all_goals
+        apply ih ‹_›
+
+instance [Iterator α Id β] [LawfulDeterministicIterator α Id] {it : IterM (α := α) Id β} :
+    Subsingleton (PlausibleIterStep (it.IsPlausibleNthOutputStep n)) where
+  allEq s s' := by
+    obtain ⟨s, hs⟩ := s
+    obtain ⟨s', hs'⟩ := s'
+    have := IterM.eq_of_isPlausibleNthOutputStep_of_isPlausibleNthOutputStep hs hs'
+    rwa [Subtype.mk.injEq]
+
+theorem _root_.Std.IterM.step_stepSize [Iterator α Id β] [Productive α Id] [LawfulDeterministicIterator α Id]
+    [IteratorAccess α Id] {it : IterM (α := α) Id β} {n : Nat} :
+    it.nextAtIdx? n = it.nextAtIdxSlow? n := by
+  ext
+  apply Subsingleton.allEq
+
+theorem step_stepSize [Iterator α Id β] [Productive α Id] [LawfulDeterministicIterator α Id]
+    [IteratorAccess α Id] {it : Iter (α := α) β} {n : Nat} :
+    it.nextAtIdx? n = it.nextAtIdxSlow? n := by
+  simp [Iter.nextAtIdx?, Iter.nextAtIdxSlow?, IterM.step_stepSize]
+
+theorem atIdxSlow?_stepSize_aux [Iterator α Id β] [Productive α Id] [LawfulDeterministicIterator α Id]
+    [IteratorAccess α Id] {it : Iter (α := α) β} {n : Nat} :
+    (Iter.Intermediate.stepSize it i n).atIdxSlow? k = it.atIdxSlow? (i + (n - 1 + 1) * k) := by
+  induction k
+  · simp
+    induction i, it using Iter.atIdxSlow?.induct_unfolding
+    case yield_zero it it' _ h _ =>
+      rw [atIdxSlow?_eq_match]
+      simp [Intermediate.stepSize, IterM.Intermediate.stepSize, Iter.step_eq]
+      cases (it.toIterM.nextAtIdx? 0).run using PlausibleIterStep.casesOn
+      · rename_i h'
+        simp [Iter.IsPlausibleStep] at h
+        replace h := IterM.IsPlausibleNthOutputStep.zero_yield h
+        cases IterM.eq_of_isPlausibleNthOutputStep_of_isPlausibleNthOutputStep h h'
+        simp
+      · rename_i h'
+        simp [Iter.IsPlausibleStep] at h
+        replace h := IterM.IsPlausibleNthOutputStep.zero_yield h
+        cases IterM.eq_of_isPlausibleNthOutputStep_of_isPlausibleNthOutputStep h h'
+      · rename_i h'
+        simp [Iter.IsPlausibleStep] at h
+        replace h := IterM.IsPlausibleNthOutputStep.zero_yield h
+        cases IterM.eq_of_isPlausibleNthOutputStep_of_isPlausibleNthOutputStep h h'
+    case yield_succ it it' _ h _ =>
+      rw [atIdxSlow?_eq_match, atIdxSlow?_eq_match]
+  generalize h : Iter.Intermediate.stepSize it i n = sit
+  induction k, sit using Iter.atIdxSlow?.induct_unfolding
+  case yield_zero =>
+    simp
+    simp [Intermediate.stepSize, IterM.Intermediate.stepSize] at h
+
+theorem atIdxSlow?_stepSize [Iterator α Id β] [Productive α Id] [LawfulDeterministicIterator α Id]
+    [IteratorAccess α Id] {it : Iter (α := α) β} {n : Nat} :
+    (it.stepSize n).atIdxSlow? k = it.atIdxSlow? ((n - 1 + 1) * k) := by
+
+
+end Std.Iter
